src/ml/libvellvm/interpreter.mli
@@ -1,14 +1,18 @@
-;; open TopLevel.IO
+open Handlers.Mem
+open Handlers.Local
+open Handlers.Stack
+open Handlers.Global
+open Handlers.LLVMEvents
 open ITreeDefinition
 
-val pp_addr : Format.formatter -> Memory.A.addr -> unit
+val pp_addr : Format.formatter -> Memory.Addr.addr -> unit
 
 val pp_uvalue : Format.formatter -> DV.uvalue -> unit
 
 val interpret: ((LLVMAst.typ, LLVMAst.typ LLVMAst.block * (LLVMAst.typ LLVMAst.block) list) LLVMAst.toplevel_entity) list -> (DV.uvalue, string) result
 
 (* SAZ: do we need to expose the step function in this way?  Its type is very complicated *)
-(* val step : ((Obj.t Std.failureE, Obj.t debugE, 'b) Sum.sum1, DV.dvalue) coq_LLVM -> (TopLevel.IO.DV.dvalue, string) result *)
-val step : ('a TopLevel.IO.coq_L5, TopLevel.TopLevelEnv.memory * ((TopLevel.TopLevelEnv.local_env * TopLevel.TopLevelEnv.stack) * (TopLevel.TopLevelEnv.global_env * TopLevel.IO.DV.uvalue))) itree -> (TopLevel.IO.DV.uvalue, string) result
+(* val step : ((Obj.t Std.failureE, Obj.t debugE, 'b) Sum.sum1, DV.dvalue) coq_LLVM -> (TopLevel.LLVMEvents.DV.dvalue, string) result *)
+val step : ('a coq_L5, memory_stack * ((local_env * lstack) * (global_env * DV.uvalue))) itree -> (DV.uvalue, string) result
 
 val debug_flag: bool ref
