src/coq/Refinement.v
@@ -11,16 +11,14 @@ From Vellvm Require Import
      LLVMEvents
      LLVMAst
      Environment
-     Handlers.Stack.
+     Handlers.Handlers.
 
 From Coq Require Import Relations RelationClasses.
 
+Module Make (A:MemoryAddress.ADDRESS)(LLVMEvents: LLVM_INTERACTIONS(A)).
 
-Module Make(A:MemoryAddress.ADDRESS)(LLVMIO: LLVM_INTERACTIONS(A))(ENV: Environment).
-
-Import LLVMIO.
-Import LLVMIO.DV.
-Import ENV.
+Import LLVMEvents.
+Import DV.
 
 (* Refinement relation for uvalues *)
 Inductive refine_uvalue: uvalue -> uvalue -> Prop :=
@@ -63,21 +61,21 @@ Definition refine_L1 : relation (itree L1 (global_env * uvalue))
   := eutt refine_res1.
 
 (* Refinement of mcfg after locals *)
-Definition refine_res2 : relation (local_env * stack * (global_env * uvalue))
+Definition refine_res2 : relation (local_env * lstack * (global_env * uvalue))
   := TT × refine_res1.
 
 Definition refine_L2 : relation (itree L2 (local_env * stack * (global_env * uvalue)))
   := eutt refine_res2.
 
 (* For multiple CFG, after interpreting [LocalE] and [MemoryE] and [IntrinsicE] that are memory intrinsics *)
-Definition refine_res3 : relation (memory * (local_env * stack * (global_env * uvalue)))
+Definition refine_res3 : relation (memory_stack * (local_env * stack * (global_env * uvalue)))
   := TT × refine_res2.
 
-Definition refine_L3 : relation (itree L3 (memory * (local_env * stack * (global_env * uvalue))))
+Definition refine_L3 : relation (itree L3 (memory_stack * (local_env * stack * (global_env * uvalue))))
   := eutt refine_res3.
 
 (* Refinement for after interpreting pick. *)
-Definition refine_L4 : relation ((itree L4 (memory * (local_env * stack * (global_env * uvalue)))) -> Prop)
+Definition refine_L4 : relation ((itree L4 (memory_stack * (local_env * stack * (global_env * uvalue)))) -> Prop)
   := fun ts ts' => forall t, ts t -> exists t', ts' t' /\ eutt refine_res3 t t'.
 
 (*
@@ -85,7 +83,7 @@ Definition refine_res4 : relation (memory * (local_env * stack * (global_env * d
   := TT × (TT × (TT × refine_dvalue)).
  *)
 
-Definition refine_L5 : relation ((itree L5 (memory * (local_env * stack * (global_env * uvalue)))) -> Prop)
+Definition refine_L5 : relation ((itree L5 (memory_stack * (local_env * stack * (global_env * uvalue)))) -> Prop)
   := fun ts ts' => forall t, ts t -> exists t', ts' t' /\ eutt refine_res3 t t'.
 
 End Make.
