src/coq/Handlers/Handlers.v
@@ -28,6 +28,13 @@ From Vellvm.Handlers Require Export
      UndefinedBehaviour
 .
 
+(* Handlers get instantiated over the domain of addresses provided by the memory model *)
+Module LLVMEvents := LLVMEvents.Make(Memory.Addr).
+Module Global := Global.Make Memory.Addr LLVMEvents.
+Module Local  := Local.Make  Memory.Addr LLVMEvents.
+Module Stack  := Stack.Make  Memory.Addr LLVMEvents.
+Module Intrinsics := Intrinsics.Make Memory.Addr LLVMEvents.
+Module Mem := Memory.Make LLVMEvents.
+Module Pick := Pick.Make Memory.Addr LLVMEvents.
 
-
-
+Export LLVMEvents LLVMEvents.DV Global Local Stack Mem Pick Intrinsics UndefinedBehaviour.       
