src/coq/Handlers/Local.v
@@ -13,10 +13,6 @@ From ITree Require Import
 
 From Vellvm Require Import
      Util
-     LLVMAst
-     AstLib
-     MemoryAddress
-     DynamicValues
      LLVMEvents
      Error.
 
@@ -146,3 +142,20 @@ Section Locals.
   End PARAMS.
 
 End Locals.
+
+From ExtLib Require Import
+     Data.Map.FMapAList.
+From Vellvm Require Import
+     LLVMAst
+     MemoryAddress.
+
+(* YZ TODO : Undecided about the status of this over-generalization of these events over domains of keys and values.
+   The interface needs to be specialized anyway in [LLVMEvents].
+   We want to have access to the specialized type both in [InterpreterMCFG] and [InterpreterCFG] so we cannot delay
+   it until [TopLevel] either.
+   So exposing the specialization here, but it is awkward.
+ *)
+Module Make (A : ADDRESS) (LLVMEvents : LLVM_INTERACTIONS(A)).
+  Definition local_env := FMapAList.alist raw_id LLVMEvents.DV.uvalue.
+End Make.
+
