src/coq/InterpreterCFG.v
@@ -1,0 +1,234 @@
+From Coq Require Import
+     Morphisms.
+
+From ITree Require Import
+     ITree
+     Basics.Monad
+     Eq.Eq.
+
+From Vellvm Require Import
+     LLVMEvents
+     Handlers.Handlers.
+
+Section InterpreterCFG.
+
+  (**
+   Partial interpretations of the trees produced by the
+   denotation of cfg. They differ from the ones of Vellvm programs by
+   their event signature, as well as by the lack of a stack of local event.
+   The intent is to allow us to only interpret as many layers as needed
+   to perform the required semantic reasoning, and lift for free the
+   equivalence down the pipe.
+   This gives us a _vertical_ notion of compositionality.
+   *)
+
+  (**
+   NOTE: Can we avoid this duplication w.r.t. [interp_to_Li]?
+   *)
+
+  Definition interp_cfg_to_L1 {R} user_intrinsics (t: itree instr_E R) (g: global_env) :=
+    let L0_trace       := interp_intrinsics user_intrinsics t in
+    let L1_trace       := interp_global L0_trace g in
+    L1_trace.
+
+  Definition interp_cfg_to_L2 {R} user_intrinsics (t: itree instr_E R) (g: global_env) (l: local_env) :=
+    let L0_trace       := interp_intrinsics user_intrinsics t in
+    let L1_trace       := interp_global L0_trace g in
+    let L2_trace       := interp_local L1_trace l in
+    L2_trace.
+
+  Definition interp_cfg_to_L3 {R} user_intrinsics (t: itree instr_E R) (g: global_env) (l: local_env) (m: memory_stack) :=
+    let L0_trace       := interp_intrinsics user_intrinsics t in
+    let L1_trace       := interp_global L0_trace g in
+    let L2_trace       := interp_local L1_trace l in
+    let L3_trace       := interp_memory L2_trace m in
+    L3_trace.
+
+  Definition interp_cfg_to_L4 {R} user_intrinsics (t: itree instr_E R) (g: global_env) (l: local_env) (m: memory_stack) :=
+    let L0_trace       := interp_intrinsics user_intrinsics t in
+    let L1_trace       := interp_global L0_trace g in
+    let L2_trace       := interp_local L1_trace l in
+    let L3_trace       := interp_memory L2_trace m in
+    let L4_trace       := model_undef L3_trace in
+    L4_trace.
+
+  Definition interp_cfg_to_L5 {R} user_intrinsics (t: itree instr_E R) (g: global_env) (l: local_env) (m: memory_stack) :=
+    let L0_trace       := interp_intrinsics user_intrinsics t in
+    let L1_trace       := interp_global L0_trace g in
+    let L2_trace       := interp_local L1_trace l in
+    let L3_trace       := interp_memory L2_trace m in
+    let L4_trace       := model_undef L3_trace in
+    model_UB L4_trace.
+
+  Lemma interp_cfg_to_L1_bind :
+    forall ui {R S} (t: itree instr_E R) (k: R -> itree instr_E S) g, 
+      interp_cfg_to_L1 ui (ITree.bind t k) g ≈
+                       (ITree.bind (interp_cfg_to_L1 ui t g) (fun '(g',x) => interp_cfg_to_L1 ui (k x) g')).
+  Proof.
+    intros.
+    unfold interp_cfg_to_L1.
+    rewrite interp_intrinsics_bind, interp_global_bind.
+    apply eutt_eq_bind; intros (? & ?); reflexivity.
+  Qed.
+
+  Lemma interp_cfg_to_L1_ret : forall ui (R : Type) g (x : R), interp_cfg_to_L1 ui (Ret x) g ≈ Ret (g,x).
+  Proof.
+    intros; unfold interp_cfg_to_L1.
+    rewrite interp_intrinsics_ret, interp_global_ret; reflexivity.
+  Qed.
+
+  Lemma interp_cfg_to_L2_bind :
+    forall ui {R S} (t: itree instr_E R) (k: R -> itree instr_E S) g l,
+      interp_cfg_to_L2 ui (ITree.bind t k) g l ≈
+                       (ITree.bind (interp_cfg_to_L2 ui t g l) (fun '(g',(l',x)) => interp_cfg_to_L2 ui (k x) l' g')).
+  Proof.
+    intros.
+    unfold interp_cfg_to_L2.
+    rewrite interp_intrinsics_bind, interp_global_bind, interp_local_bind.
+    apply eutt_eq_bind; intros (? & ? & ?); reflexivity.
+  Qed.
+
+  Lemma interp_cfg_to_L2_ret : forall ui (R : Type) g l (x : R), interp_cfg_to_L2 ui (Ret x) g l ≈ Ret (l, (g, x)).
+  Proof.
+    intros; unfold interp_cfg_to_L2.
+    rewrite interp_intrinsics_ret, interp_global_ret, interp_local_ret; reflexivity.
+  Qed.
+
+  Lemma interp_cfg_to_L3_bind :
+    forall ui {R S} (t: itree instr_E R) (k: R -> itree instr_E S) g l m,
+      interp_cfg_to_L3 ui (ITree.bind t k) g l m ≈
+                       (ITree.bind (interp_cfg_to_L3 ui t g l m) (fun '(m',(l',(g',x))) => interp_cfg_to_L3 ui (k x) g' l' m')).
+  Proof.
+    intros.
+    unfold interp_cfg_to_L3.
+    rewrite interp_intrinsics_bind, interp_global_bind, interp_local_bind, interp_memory_bind.
+    apply eutt_eq_bind; intros (? & ? & ? & ?); reflexivity.
+  Qed.
+
+  Lemma interp_cfg_to_L3_ret : forall ui (R : Type) g l m (x : R), interp_cfg_to_L3 ui (Ret x) g l m ≈ Ret (m, (l, (g,x))).
+  Proof.
+    intros; unfold interp_cfg_to_L3.
+    rewrite interp_intrinsics_ret, interp_global_ret, interp_local_ret, interp_memory_ret; reflexivity.
+  Qed.
+
+  Global Instance eutt_interp_cfg_to_L1 (defs: intrinsic_definitions) {T}:
+    Proper (eutt Logic.eq ==> Logic.eq ==> eutt Logic.eq) (@interp_cfg_to_L1 T defs).
+  Proof.
+    repeat intro.
+    unfold interp_cfg_to_L1.
+    subst; rewrite H.
+    reflexivity.
+  Qed.
+
+  Global Instance eutt_interp_cfg_to_L2 (defs: intrinsic_definitions) {T}:
+    Proper (eutt Logic.eq ==> Logic.eq ==> Logic.eq ==> eutt Logic.eq) (@interp_cfg_to_L2 T defs).
+  Proof.
+    repeat intro.
+    unfold interp_cfg_to_L2.
+    subst; rewrite H.
+    reflexivity.
+  Qed.
+
+  Global Instance eutt_interp_cfg_to_L3 (defs: intrinsic_definitions) {T}:
+    Proper (eutt Logic.eq ==> Logic.eq ==> Logic.eq ==> Logic.eq ==> eutt Logic.eq) (@interp_cfg_to_L3 T defs).
+  Proof.
+    repeat intro.
+    unfold interp_cfg_to_L3.
+    subst; rewrite H.
+    reflexivity.
+  Qed.
+
+  (* NOTEYZ: This can probably be refined to [eqit eq] instead of [eutt eq], but I don't think it matters to us *)
+  Lemma interp_cfg_to_L3_vis (defs: IS.intrinsic_definitions):
+    forall T R (e : instr_E T) (k : T -> itree instr_E R) g l m,
+      interp_cfg_to_L3 defs (Vis e k) g l m ≈ 
+                       ITree.bind (interp_cfg_to_L3 defs (trigger e) g l m)
+                       (fun '(m, (l, (g, x)))=> interp_cfg_to_L3 defs (k x) g l m).
+  Proof.
+    intros.
+    unfold interp_cfg_to_L3.
+    rewrite interp_intrinsics_vis.
+    rewrite interp_global_bind, interp_local_bind, interp_memory_bind.
+    unfold trigger; rewrite interp_intrinsics_vis.
+    rewrite interp_global_bind, interp_local_bind, interp_memory_bind.
+    rewrite Eq.bind_bind.
+    apply eutt_eq_bind.
+    intros (? & ? & ? & ?).
+    do 2 match goal with
+      |- context[interp ?x ?t] => replace (interp x t) with (interp_intrinsics defs t) by reflexivity
+    end. 
+    rewrite interp_intrinsics_ret, interp_global_ret, interp_local_ret, interp_memory_ret, bind_ret_l.
+    reflexivity.
+  Qed.
+
+  Lemma interp_cfg_to_L3_bind_trigger (defs: IS.intrinsic_definitions):
+    forall T R (e : instr_E T) (k : T -> itree instr_E R) g l m,
+      interp_cfg_to_L3 defs (ITree.bind (trigger e) k) g l m ≈ 
+                       ITree.bind (interp_cfg_to_L3 defs (trigger e) g l m)
+                       (fun '(m, (l, (g, x)))=> interp_cfg_to_L3 defs (k x) g l m).
+  Proof.
+    intros.
+    rewrite bind_trigger.
+    rewrite interp_cfg_to_L3_vis at 1.
+    reflexivity.
+  Qed.
+
+  Lemma interp_cfg_to_L3_GR : forall defs id g l m v,
+      Maps.lookup id g = Some v ->
+      interp_cfg_to_L3 defs (trigger (GlobalRead id)) g l m ≈ ret (m,(l,(g,v))).
+  Proof.
+    intros * LU.
+    unfold interp_cfg_to_L3.
+    rewrite interp_intrinsics_trigger.
+    cbn.
+    unfold Intrinsics.F_trigger.
+    rewrite interp_global_trigger.
+    cbn in *; rewrite LU.
+    rewrite interp_local_ret, interp_memory_ret.
+    reflexivity.
+  Qed.
+
+  Lemma interp_cfg_to_L3_LR : forall defs id g l m v,
+      Maps.lookup id l = Some v ->
+      interp_cfg_to_L3 defs (trigger (LocalRead id)) g l m ≈ ret (m,(l,(g,v))).
+  Proof.
+    intros * LU.
+    unfold interp_cfg_to_L3.
+    rewrite interp_intrinsics_trigger.
+    cbn.
+    unfold Intrinsics.F_trigger.
+    rewrite interp_global_trigger.
+    cbn.
+    rewrite interp_local_bind, interp_local_trigger.
+    cbn in *; rewrite LU.
+    rewrite bind_ret_l, interp_local_ret, interp_memory_ret.
+    reflexivity.
+  Qed.
+
+  (**
+     TODO YZ: Can we expose better than this? It's super low level
+   *)
+  Lemma interp_cfg_to_L3_LM : forall defs t a size offset g l m v bytes concrete_id,
+      lookup_logical a (fst m) = Some (LBlock size bytes concrete_id) ->
+      deserialize_sbytes (lookup_all_index offset (sizeof_dtyp t) bytes SUndef) t = v ->
+      interp_cfg_to_L3 defs (trigger (Load t (DVALUE_Addr (a, offset)))) g l m ≈ Ret (m,(l,(g,v))).
+  Proof.
+    intros * LUL EQ.
+    unfold interp_cfg_to_L3.
+    rewrite interp_intrinsics_trigger.
+    cbn.
+    unfold Intrinsics.F_trigger.
+    rewrite interp_global_trigger.
+    cbn.
+    rewrite interp_local_bind, interp_local_trigger.
+    cbn; rewrite bind_bind.
+    rewrite interp_memory_bind, interp_memory_trigger.
+    cbn.
+    destruct m as [mem memstack]. cbn.
+    cbn in LUL; rewrite LUL.
+    rewrite 2 bind_ret_l, interp_local_ret, interp_memory_ret.
+    rewrite EQ.
+    reflexivity.
+  Qed.
+
+End InterpreterCFG.
