src/coq/InterpreterMCFG.v
@@ -1,0 +1,235 @@
+From Coq Require Import
+     Morphisms.
+
+From ITree Require Import
+     ITree
+     Basics.Monad
+     Eq.Eq.
+
+From Vellvm Require Import
+     LLVMEvents
+     Handlers.Handlers.
+
+Section InterpreterMCFG.
+
+  (**
+   Partial interpretations of the trees produced by the denotation of _VIR_ programs.
+   The intent is to allow us to only interpret as many layers as needed
+   to perform the required semantic reasoning, and lift for free the
+   equivalence down the pipe.
+   This gives us a _vertical_ notion of compositionality.
+   *)
+
+  Definition interp_to_L1 {R} user_intrinsics (t: itree L0 R) g :=
+    let uvalue_trace       := interp_intrinsics user_intrinsics t in
+    let L1_trace           := interp_global uvalue_trace g in
+    L1_trace.
+
+  Definition interp_to_L2 {R} user_intrinsics (t: itree L0 R) g l :=
+    let uvalue_trace   := interp_intrinsics user_intrinsics t in
+    let L1_trace       := interp_global uvalue_trace g in
+    let L2_trace       := interp_local_stack (handle_local (v:=uvalue)) L1_trace l in
+    L2_trace.
+
+  Definition interp_to_L3 {R} user_intrinsics (t: itree L0 R) g l m :=
+    let uvalue_trace   := interp_intrinsics user_intrinsics t in
+    let L1_trace       := interp_global uvalue_trace g in
+    let L2_trace       := interp_local_stack (handle_local (v:=uvalue)) L1_trace l in
+    let L3_trace       := interp_memory L2_trace m in
+    L3_trace.
+
+  Definition interp_to_L4 {R} user_intrinsics (t: itree L0 R) g l m :=
+    let uvalue_trace   := interp_intrinsics user_intrinsics t in
+    let L1_trace       := interp_global uvalue_trace g in
+    let L2_trace       := interp_local_stack (handle_local (v:=uvalue)) L1_trace l in
+    let L3_trace       := interp_memory L2_trace m in
+    let L4_trace       := model_undef L3_trace in
+    L4_trace.
+
+  Definition interp_to_L5 {R} user_intrinsics (t: itree L0 R) g l m :=
+    let uvalue_trace   := interp_intrinsics user_intrinsics t in
+    let L1_trace       := interp_global uvalue_trace g in
+    let L2_trace       := interp_local_stack (handle_local (v:=uvalue)) L1_trace l in
+    let L3_trace       := interp_memory L2_trace m in
+    let L4_trace       := model_undef L3_trace in
+    model_UB L4_trace.
+
+  (* The interpreter stray away from the model starting from the fourth layer: we pick an arbitrary valid path of execution *)
+  Definition interp_to_L4_exec {R} user_intrinsics (t: itree L0 R) g l m :=
+    let uvalue_trace   := interp_intrinsics user_intrinsics t in
+    let L1_trace       := interp_global uvalue_trace g in
+    let L2_trace       := interp_local_stack (handle_local (v:=uvalue)) L1_trace l in
+    let L3_trace       := interp_memory L2_trace m in
+    let L4_trace       := exec_undef L3_trace in
+    L4_trace.
+
+  Definition interp_to_L5_exec {R} user_intrinsics (t: itree L0 R) g l m :=
+    let uvalue_trace   := interp_intrinsics user_intrinsics t in
+    let L1_trace       := interp_global uvalue_trace g in
+    let L2_trace       := interp_local_stack (handle_local (v:=uvalue)) L1_trace l in
+    let L3_trace       := interp_memory L2_trace m in
+    let L4_trace       := exec_undef L3_trace in
+    exec_UB L4_trace.
+
+  Section Structural_Lemmas.
+
+    Lemma interp_to_L1_bind :
+      forall ui {R S} (t: itree L0 R) (k: R -> itree L0 S) g, 
+        interp_to_L1 ui (ITree.bind t k) g ≈
+                     (ITree.bind (interp_to_L1 ui t g) (fun '(g',x) => interp_to_L1 ui (k x) g')).
+    Proof.
+      intros.
+      unfold interp_to_L1.
+      rewrite interp_intrinsics_bind, interp_global_bind.
+      apply eutt_eq_bind; intros (? & ?); reflexivity.
+    Qed.
+
+    Lemma interp_to_L1_ret : forall ui (R : Type) g (x : R), interp_to_L1 ui (Ret x) g ≈ Ret (g,x).
+    Proof.
+      intros; unfold interp_to_L1.
+      rewrite interp_intrinsics_ret, interp_global_ret; reflexivity.
+    Qed.
+
+    Lemma interp_to_L2_bind :
+      forall ui {R S} (t: itree L0 R) (k: R -> itree L0 S) g l,
+        interp_to_L2 ui (ITree.bind t k) g l ≈
+                     (ITree.bind (interp_to_L2 ui t g l) (fun '(g',(l',x)) => interp_to_L2 ui (k x) l' g')).
+    Proof.
+      intros.
+      unfold interp_to_L2.
+      rewrite interp_intrinsics_bind, interp_global_bind, interp_local_stack_bind.
+      apply eutt_eq_bind; intros (? & ? & ?); reflexivity.
+    Qed.
+
+    Lemma interp_to_L2_ret : forall ui (R : Type) g l (x : R), interp_to_L2 ui (Ret x) g l ≈ Ret (l, (g, x)).
+    Proof.
+      intros; unfold interp_to_L2.
+      rewrite interp_intrinsics_ret, interp_global_ret, interp_local_stack_ret; reflexivity.
+    Qed.
+
+    Lemma interp_to_L3_bind :
+      forall ui {R S} (t: itree L0 R) (k: R -> itree L0 S) g l m,
+        interp_to_L3 ui (ITree.bind t k) g l m ≈
+                     (ITree.bind (interp_to_L3 ui t g l m) (fun '(m',(l',(g',x))) => interp_to_L3 ui (k x) g' l' m')).
+    Proof.
+      intros.
+      unfold interp_to_L3.
+      rewrite interp_intrinsics_bind, interp_global_bind, interp_local_stack_bind, interp_memory_bind.
+      apply eutt_eq_bind; intros (? & ? & ? & ?); reflexivity.
+    Qed.
+
+    Lemma interp_to_L3_ret : forall ui (R : Type) g l m (x : R), interp_to_L3 ui (Ret x) g l m ≈ Ret (m, (l, (g,x))).
+    Proof.
+      intros; unfold interp_to_L3.
+      rewrite interp_intrinsics_ret, interp_global_ret, interp_local_stack_ret, interp_memory_ret; reflexivity.
+    Qed.
+
+    Global Instance eutt_interp_to_L1 (defs: intrinsic_definitions) {T}:
+      Proper (eutt Logic.eq ==> Logic.eq ==> eutt Logic.eq) (@interp_to_L1 T defs).
+    Proof.
+      repeat intro.
+      unfold interp_to_L1.
+      subst; rewrite H.
+      reflexivity.
+    Qed.
+
+    Global Instance eutt_interp_to_L2 (defs: intrinsic_definitions) {T}:
+      Proper (eutt Logic.eq ==> Logic.eq ==> Logic.eq ==> eutt Logic.eq) (@interp_to_L2 T defs).
+    Proof.
+      repeat intro.
+      unfold interp_to_L2.
+      subst; rewrite H.
+      reflexivity.
+    Qed.
+
+    Global Instance eutt_interp_to_L3 (defs: intrinsic_definitions) {T}:
+      Proper (eutt Logic.eq ==> Logic.eq ==> Logic.eq ==> Logic.eq ==> eutt Logic.eq) (@interp_to_L3 T defs).
+    Proof.
+      repeat intro.
+      unfold interp_to_L3.
+      subst; rewrite H.
+      reflexivity.
+    Qed.
+
+    (* NOTEYZ: This can probably be refined to [eqit eq] instead of [eutt eq], but I don't think it matters to us *)
+    Lemma interp_to_L3_vis (defs: IS.intrinsic_definitions):
+      forall T R (e : L0 T) (k : T -> itree L0 R) g l m,
+        interp_to_L3 defs (Vis e k) g l m ≈ 
+                     ITree.bind (interp_to_L3 defs (trigger e) g l m)
+                     (fun '(m, (l, (g, x)))=> interp_to_L3 defs (k x) g l m).
+    Proof.
+      intros.
+      unfold interp_to_L3.
+      rewrite interp_intrinsics_vis.
+      rewrite interp_global_bind, interp_local_stack_bind, interp_memory_bind.
+      unfold trigger; rewrite interp_intrinsics_vis.
+      rewrite interp_global_bind, interp_local_stack_bind, interp_memory_bind.
+      rewrite Eq.bind_bind.
+      apply eutt_eq_bind.
+      intros (? & ? & ? & ?).
+      do 2 match goal with
+             |- context[interp ?x ?t] => replace (interp x t) with (interp_intrinsics defs t) by reflexivity
+           end. 
+      rewrite interp_intrinsics_ret, interp_global_ret, interp_local_stack_ret, interp_memory_ret, bind_ret_l.
+      reflexivity.
+    Qed.
+
+    Lemma interp_to_L3_bind_trigger (defs: IS.intrinsic_definitions):
+      forall T R (e : L0 T) (k : T -> itree L0 R) g l m,
+        interp_to_L3 defs (ITree.bind (trigger e) k) g l m ≈ 
+                     ITree.bind (interp_to_L3 defs (trigger e) g l m)
+                     (fun '(m, (l, (g, x)))=> interp_to_L3 defs (k x) g l m).
+    Proof.
+      intros.
+      rewrite bind_trigger.
+      rewrite interp_to_L3_vis at 1.
+      reflexivity.
+    Qed.
+
+  End Structural_Lemmas.
+
+End InterpreterMCFG.
+
+Ltac fold_L1 :=
+  match goal with
+    |- context[interp_global (interp_intrinsics ?ui ?p) ?g] =>
+    replace (interp_global (interp_intrinsics ui p) g) with
+    (interp_to_L1 ui p g) by reflexivity
+  end.
+
+Ltac fold_L2 :=
+  match goal with
+    |- context[interp_local_stack ?h
+                                 (interp_global (interp_intrinsics ?ui ?p) ?g) ?l] =>
+    replace (interp_local_stack h (interp_global (interp_intrinsics ui p) g) l) with
+    (interp_to_L2 ui p g l) by reflexivity
+  end.
+
+Ltac fold_L3 :=
+  match goal with
+    |- context[
+          interp_memory
+            (interp_local_stack ?h
+                                (interp_global (interp_intrinsics ?ui ?p) ?g) ?l) ?m] =>
+    replace (interp_memory (interp_local_stack h (interp_global (interp_intrinsics ui p) g) l) m) with
+    (interp_to_L3 ui p g l m) by reflexivity
+  end.
+
+Ltac fold_L4 :=
+  match goal with
+    |- context[
+          model_undef
+            (interp_memory
+               (interp_local_stack ?h
+                                   (interp_global (interp_intrinsics ?ui ?p) ?g) ?l) ?m)] =>
+    replace (model_undef (interp_memory (interp_local_stack h (interp_global (interp_intrinsics ui p) g) l) m)) with
+    (interp_to_L4 ui p g l m) by reflexivity
+  end.
+
+Ltac fold_L5 :=
+  match goal with
+    |- context[model_UB (model_undef (interp_memory (interp_local_stack ?h (interp_global (interp_intrinsics ?ui ?p) ?g) ?l) ?m))] =>
+    replace (model_UB (model_undef (interp_memory (interp_local_stack h (interp_global (interp_intrinsics ui p) g) l) m))) with
+    (interp_to_L5 ui p g l m) by reflexivity
+  end.
+
